backends/lean/Base/List.lean
@@ -1,1 +1,1 @@
-import Base.IList.IList
+import Base.List.List
