backends/lean/Base/Primitives/CoreConvertNum.lean
@@ -2,7 +2,6 @@ import Lean
 import Lean.Meta.Tactic.Simp
 import Init.Data.List.Basic
 import Mathlib.Tactic.Linarith
-import Base.IList
 import Base.Primitives.Scalar
 import Base.Primitives.ScalarNotations
 import Base.Primitives.ArraySlice
